theories/cap_lang.v
@@ -808,6 +808,9 @@ Section opsem.
   | FailedV: val
   | NextIV: val.
 
+Global Instance instr_eq_val : EqDecision val.
+Proof. solve_decision. Defined.
+
   (* TODO: change to co-inductive list in the Seq case *)
   Inductive expr: Type :=
   | Instr (c : ConfFlag)
